feat: reverse `HashMap.toList`, so it agrees with `HashMap.toArray` (#6244)
This PR changes the implementation of `HashMap.toList`, so the ordering
agrees with `HashMap.toArray`.

Currently there are no verification lemmas about `HashMap.toList`, so no
contract is being broken yet!

src/Std/Data/DHashMap/Internal/AssocList/Basic.lean
@@ -10,6 +10,11 @@ import Init.NotationExtra
 This is an internal implementation file of the hash map. Users of the hash map should not rely on
 the contents of this file.
 
+Note that some functions in this file (in particular, `foldrM`, `foldr`, `toList`, `replace`, and
+`erase`) are not tail-recursive. This is not a problem because they are only used internally by
+`HashMap`, where `AssocList` is always small. Before making this API public, we would need to add
+`@[csimp]` lemmas for tail-recursive implementations.
+
 File contents: Operations on associative lists
 -/
 
@@ -45,6 +50,17 @@ namespace AssocList
 /-- Internal implementation detail of the hash map -/
 @[inline] def foldl (f : δ → (α : α) → β α → δ) (init : δ) (as : AssocList α β) : δ :=
   Id.run (foldlM f init as)
+
+/-- Internal implementation detail of the hash map -/
+@[specialize] def foldrM (f : (a : α) → β a → δ → m δ) : (init : δ) → AssocList α β → m δ
+  | d, nil         => pure d
+  | d, cons a b es => do
+    let d ← foldrM f d es
+    f a b d
+
+/-- Internal implementation detail of the hash map -/
+@[inline] def foldr (f : (a : α) → β a → δ → δ) (init : δ) (as : AssocList α β) : δ :=
+  Id.run (foldrM f init as)
 
 /-- Internal implementation detail of the hash map -/
 @[inline] def forM (f : (a : α) → β a → m PUnit) (as : AssocList α β) : m PUnit :=
